<?xml version="1.0" encoding="UTF-8"?>
<!-- Generated by Pandoc using pretext.lua -->


<section xml:id="sec-complexNums">
	<title>Complex Numbers</title>

	<p> The equation <m>x^{2} + 1 = 0</m> has no real number solutions. However, it <em>would</em>
		have solutions if we could make sense of <m>\sqrt{-1}</m>. The <em>Complex Numbers</em> do
		just that - they give us a mechanism for working with <m>\sqrt{-1}</m>. As such, the set of
		complex numbers fill in an algebraic gap left by the set of real numbers. </p>

	<p> Here’s the basic plan. There is no real number <m>x</m> with <m>x^2 = -1</m>, since for any
		real number <m>x^2 \geq 0</m>. However, we could formally extract square roots and write <m>x
		= \pm \sqrt{-1}</m>. We build the complex numbers by relabeling the quantity <m>\sqrt{-1}</m>
		as <m>i</m>, the unfortunately misnamed <em>imaginary unit</em>.<fn>
			 Some Technical Mathematics textbooks label it <sq>
					<m>j</m>
				</sq>. While it carries the adjective <sq>imaginary</sq>,
		these numbers have essential real-world implications. For example, every electronic device
		owes its existence to the study of <sq>imaginary</sq> numbers. 
		</fn> The number <m>
		i</m>, while not a real number, is defined so that it plays along well with real numbers and
		acts very much like any other radical expression. For instance, <m>3(2i) = 6i</m>, <m>7i-3i
		= 4i</m>, <m>(2-7i) + (3 + 4i) = 5-3i</m>, and so forth. The key properties which
		distinguish <m>i</m> from the real numbers are listed below. </p>

	<!-- div attr= class="definition"-->
	<p> The imaginary unit <m>i</m> satisfies the two following properties: </p>

	<p>
		<ol>
			<li>
				<p>
					<m>i^2 = -1</m>
				</p>
			</li>

			<li>
				<p> If <m>c</m> is a real number with <m>c \geq 0</m> then <m>\sqrt{-c} = i \sqrt{c}</m>
				</p>
			</li>

		</ol>
	</p><!--</div
	attr= class="definition">-->

	<p> Property 1 in the previous definition establishes that <m>i</m> does act as a square root<fn>
			 Note the use of the indefinite article <sq>a</sq>. Whatever beast is chosen to be <m>
		i</m>, <m>-i</m> is the other square root of <m>-1</m>. 
		</fn> of <m>-1</m>, and
		property 2 establishes what we mean by the <sq>principal square root</sq> of a negative real
		number. In property 2, it is important to remember the restriction on <m>c</m>. For example,
		it is perfectly acceptable to say <m>\sqrt{-4} = i \sqrt{4} = i(2) = 2i</m>. However, <m>\sqrt{-(-4)}
		\neq i \sqrt{-4}</m>, otherwise, we’d get<me>2 = \sqrt{4} = \sqrt{-(-4)} = i \sqrt{-4} = i
		(2i) = 2i^2 = 2(-1) = -2,</me> which is unacceptable. The moral of this story is that the
		general properties of radicals do not apply for even roots of negative quantities. With
		Definition <xref ref="idefn" /> in place, we can define the set of <em>complex numbers</em>. </p>

	<p> A <em>complex number</em> is a number of the form <m>a+bi</m>, where <m>a</m> and <m>b</m>
		are real numbers and <m>i</m> is the imaginary unit. The set of complex numbers is denoted <m>
		\C</m>. </p>

	<p> Complex numbers include things you’d normally expect, like <m>3+2i</m> and <m>\frac{2}{5} -
		i\sqrt{3}</m>. However, don’t forget that <m>a</m> or <m>b</m> could be zero, which means
		numbers like <m>3i</m> and <m>6</m> are also complex numbers. In other words, don’t forget
		that the complex numbers <em>include</em> the real numbers,<fn>
			 In the language of set notation, <m>\R \subseteq \C</m>. 
		</fn> so <m>0</m>
		and <m>\pi - \sqrt{21}</m> are both considered complex numbers. The arithmetic of complex
		numbers is as you would expect. The only things you need to remember are the two properties
		above. The next example should help recall how these animals behave. </p>


	<example>
		<title> </title>
		<statement>
			<p>
				Perform the indicated operations.
			</p>

			<!-- div attr= class="multicols"-->
			<p>
				3
			</p>

			<p>
				<ol>
					<li>
						<p>
							<m>(1-2i) - (3+4i)</m>
						</p>
					</li>

					<li>
						<p>
							<m>(1-2i)(3+4i)</m>
						</p>
					</li>

					<li>
						<p>
							<m>\dfrac{1-2i}{3-4i}</m>
						</p>
					</li>

				</ol>
			</p><!--</div
			attr= class="multicols">-->

			<!-- div attr= class="multicols"-->
			<p>
				3
			</p>

			<p>
				<ol>
					<li>
						<p>
							<m>\sqrt{-3} \sqrt{-12}</m>
						</p>
					</li>

					<li>
						<p>
							<m>\sqrt{(-3)(-12)}</m>
						</p>
					</li>

					<li>
						<p>
							<m>(x-[1+2i])(x-[1-2i])</m>
						</p>
					</li>

				</ol>
			</p><!--</div
			attr= class="multicols">-->
		</statement>

		<solution>
			<p>
				<ol>
					<li>
						<p> As mentioned earlier, we treat expressions involving <m>i</m> as we
							would any other radical. We distribute and combine like terms:<me>\begin{array}{rclr}
							(1-2i) - (3+4i) &amp; = &amp; 1-2i-3-4i &amp; \text{Distribute} \\
								&amp; = &amp; -2 - 6i &amp; \text{Gather like terms} \\
								\end{array}</me> Technically, we’d have to rewrite our answer <m>
							-2-6i</m> as <m>(-2) + (-6)i</m> to be (in the strictest sense) <sq>in
							the form <m>a+bi</m></sq>. That being said, even pedants have their
							limits, so <m>-2-6i</m> is good enough. </p>
					</li>

					<li>
						<p> Using the Distributive Property (a.k.a. F.O.I.L.), we get <me>\begin{array}{rclr}
							(1-2i)(3+4i) &amp; = &amp; (1)(3) + (1)(4i) - (2i)(3) - (2i)(4i) &amp;
							\text{F.O.I.L.} \\
								&amp; = &amp; 3+4i-6i-8i^2 &amp; \\
								&amp; = &amp; 3 - 2i - 8(-1) &amp; \text{$i^2=-1$} \\
								&amp; = &amp; 3 - 2i + 8 &amp; \\
								&amp; = &amp; 11 - 2i &amp; \\ \end{array}</me>
						</p>
					</li>

					<li>
						<p> How in the world are we supposed to simplify <m>\frac{1-2i}{3-4i}</m>?
							Well, we deal with the denominator <m>3-4i</m> as we would any other
							denominator containing two terms, one of which is a square root. We
							multiply both numerator and denominator by <m>3+4i</m>, the (complex)
							conjugate of <m>3 - 4i</m>. Doing so produces<me>\begin{array}{rclr}
							\dfrac{1-2i}{3-4i} &amp; = &amp; \dfrac{(1-2i)(3+4i)}{(3-4i)(3+4i)}
							&amp; \text{Equivalent Fractions} \\[8pt]

								&amp; = &amp; \dfrac{3 + 4i - 6i - 8i^2}{9 - 16i^2} &amp;
							\text{F.O.I.L.}\\[8pt]
								&amp; = &amp; \dfrac{3 - 2i - 8(-1)}{9 - 16(-1)} &amp; \text{$i^2 =
							-1$}\\[8pt]
								&amp; = &amp; \dfrac{11 - 2i}{25} &amp; \\[8pt]
								&amp; = &amp; \dfrac{11}{25} - \dfrac{2}{25} \, i &amp; \\
							\end{array}</me>
						</p>
					</li>

					<li>
						<p> We use property 2 of Definition <xref ref="idefn" /> first, then apply
							the rules of radicals applicable to real numbers to get <m>\sqrt{-3}
							\sqrt{-12} = \left(i \sqrt{3}\right) \left(i \sqrt{12}\right) = i^2
							\sqrt{3\cdot 12} = -\sqrt{36} = -6</m>. </p>
					</li>

					<li>
						<p> We adhere to the order of operations here and perform the multiplication
							before the radical to get <m>\sqrt{(-3)(-12)} = \sqrt{36} = 6</m>. </p>
					</li>

					<li>
						<p> We brute force multiply using the distributive property and find that <me>\begin{array}{rcl}
							(x-[1+2i])(x-[1-2i]) &amp; = &amp; x^2 -x[1-2i]-x[1+2i]+[1-2i][1+2i]
							\\[2pt]

								&amp; = &amp; x^2-x+2ix-x-2ix+1-2i+2i-4i^2 \\ [2pt]
								&amp; = &amp; x^2-2x + 1-4(-1)\\[2pt]
								&amp; = &amp; x^2 -2x +5 \\ \end{array}</me>
						</p>
					</li>

				</ol>
			</p>
		</solution>
	</example>
	<p> In the previous example, we used the <sq>conjugate</sq> idea from simplifying radical
		equations to divide two complex numbers. More generally, the <em>complex conjugate</em> of a
		complex number <m>a+bi</m> is the number <m>a-bi</m>. The notation commonly used for complex
		conjugation is a <sq>bar</sq>: <m>\overline{a+bi} = a-bi</m>. For example, <m>\overline{3+2i}
		= 3-2i</m> and <m>\overline{3-2i} = 3+2i</m>. To find <m>\overline{6}</m>, we note that <m>\overline{6}
		= \overline{6+0i}= 6 - 0i = 6</m>, so <m>\overline{6} = 6</m>. Similarly, <m>\overline{4i} =
		-4i</m>, since <m>\overline{4i} = \overline{0 + 4i} = 0 - 4i = -4i</m>. Note that <m>\overline{3+\sqrt{5}}
		= 3 + \sqrt{5}</m>, not <m>3 - \sqrt{5}</m>, since <m>\overline{3+\sqrt{5}} =
		\overline{3+\sqrt{5} + 0i} = 3+\sqrt{5} - 0i = 3+\sqrt{5}</m>. Here, the conjugation
		specified by the <sq>bar</sq> notation involves reversing the sign before <m>i = \sqrt{-1}</m>,
		not before <m>\sqrt{5}</m>. The properties of the conjugate are summarized in the following
		theorem. </p>

	<!-- div attr= class="theorem1"-->
	<p> Properties of the Complex Conjugate Let <m>z</m> and <m>w</m> be complex numbers. </p>

	<p>
		<ul>
			<li>
				<p>
					<m>\overline{\overline{z}} = z</m>
				</p>
			</li>

			<li>
				<p>
					<m>\overline{z+w} = \overline{z} + \overline{w}</m>
				</p>
			</li>

			<li>
				<p>
					<m>\overline{zw} = \overline{z} \, \overline{w}</m>
				</p>
			</li>

			<li>
				<p>
					<m>\overline{z^{n}} = \left(\overline{z}\right)^n</m>, for any natural number <m>
					n</m>
				</p>
			</li>

			<li>
				<p>
					<m>z</m> is a real number if and only if <m>\overline{z} = z</m>. </p>
			</li>

		</ul>
	</p><!--</div
	attr= class="theorem1">-->

	<p> Theorem <xref ref="conjugateprops" /> says in part that complex conjugation works well with
		addition, multiplication and powers. The proofs of these properties can best be achieved by
		writing out <m>z = a+bi</m> and <m>w = c+di</m> for real numbers <m>a</m>, <m>b</m>, <m>c</m>
		and <m>d</m>. Next, we compute the left and right sides of each equation and verify that
		they are the same. </p>

	<p> The proof of the first property is a very quick exercise.<fn>
			
				Trust us on this.
			
		</fn> To prove the second property, we compare <m>
		\overline{z+w}</m> with <m>\overline{z} + \overline{w}</m>. We have <m>\overline{z} +
		\overline{w} = \overline{a+bi} + \overline{c+di} = a-bi + c-di</m>. To find <m>
		\overline{z+w}</m>, we first compute <me>z+w = (a+bi) + (c+di) = (a+c)+(b+d)i</me> so <me>\overline{z+w}
		= \overline{(a+c)+(b+d)i} = (a+c) - (b+d)i = a+c - bi - di = a - bi + c - di = \overline{z}
		+ \overline{w}</me> As such, we have established <m>\overline{z+w} =
		\overline{z}+\overline{w}</m>. The proof for multiplication works similarly. The proof that
		the conjugate works well with powers can be viewed as a repeated application of the product
		rule, and is best proved using a technique called Mathematical Induction. The last property
		is a characterization of real numbers. If <m>z</m> is real, then <m>z = a + 0i</m>, so <m>\overline{z}
		= a - 0i = a = z</m>. On the other hand, if <m>z=\overline{z}</m>, then <m>a+bi = a - bi</m>
		which means <m>b=-b</m> so <m>b=0</m>. Hence, <m>z = a +0i = a</m> and is real. </p>

	<p> We now return to the business of solving quadratic equations. Consider <m>x^2-2x+5 = 0</m>.
		The discriminant <m>b^2 - 4ac = -16</m> is negative, so we know that there are no <em>real</em>
		solutions, since the Quadratic Formula would involve the term <m>\sqrt{-16}</m>. Complex
		numbers, however, are built just for such situations, so we can go ahead and apply the
		Quadratic Formula to get: <me>x = \dfrac{-(-2) \pm \sqrt{(-2)^2-4(1)(5)}}{2(1)} = \dfrac{2
		\pm \sqrt{-16}}{2} = \dfrac{2 \pm 4i}{2} = 1 \pm 2i.</me>
	</p>


	<example>
		<title> </title>
		<statement>
			<p> Find the complex solutions to the following equations.<fn>
					 Remember, all real numbers are complex numbers, so <sq>complex solutions</sq>
				means both real and non-real answers. 
				</fn>
			</p>

			<!-- div attr= class="multicols"-->
			<p>
				3
			</p>

			<p>
				<ol>
					<li>
						<p>
							<m>\dfrac{2x}{x+1} = x+3</m>
						</p>
					</li>

					<li>
						<p>
							<m>2t^4 = 9t^2 + 5</m>
						</p>
					</li>

					<li>
						<p>
							<m>z^3 + 1 = 0</m>
						</p>
					</li>

				</ol>
			</p><!--</div
			attr= class="multicols">-->
		</statement>

		<solution>
			<p>
				<ol>
					<li>
						<p> Clearing fractions yields a quadratic equation so we then proceed via
							normal quadratic equation methods. <me>\begin{array}{rclr}
							\dfrac{2x}{x+1} &amp; = &amp; x+3 &amp; \\[5pt]
								2x &amp; = &amp; (x+3)(x+1) &amp; \text{Multiply by $(x+1)$ to clear
							denominators} \\

								2x &amp; = &amp; x^2 + x + 3x + 3 &amp; \text{F.O.I.L.} \\

								2x &amp; = &amp; x^2 + 4x + 3 &amp; \text{Gather like terms} \\

								0 &amp; = &amp; x^2 + 2x + 3 &amp; \text{Subtract $2x$} \\
							\end{array}</me> From here, we apply the Quadratic Formula <me>\begin{array}{rclr}
							x &amp; = &amp; \dfrac{-2 \pm \sqrt{2^2 - 4(1)(3)}}{2(1)} &amp;
							\text{Quadratic Formula}\\[8pt]
								&amp; = &amp; \dfrac{-2 \pm \sqrt{-8}}{2} &amp;
							\text{Simplify}\\[8pt]
								&amp; = &amp; \dfrac{-2 \pm i \sqrt{8}}{2} &amp; \text{Definition of
							$i$}\\[8pt]
								&amp; = &amp; \dfrac{-2 \pm i 2\sqrt{2}}{2} &amp; \text{Product Rule
							for Radicals}\\[8pt]
								&amp; = &amp; \dfrac{\cancel{2}(-1 \pm i\sqrt{2})}{\cancel{2}} &amp;
							\text{Factor and reduce}\\[8pt]
								&amp; = &amp; -1 \pm i \sqrt{2} &amp; \\
								\end{array}</me>
						</p>

						<p> We get two answers: <m>x = -1 + i\sqrt{2}</m> and its conjugate <m>x =
							-1 - i\sqrt{2}</m>. Checking both of these answers reviews all of the
							salient points about complex number arithmetic and is therefore strongly
							encouraged. </p>
					</li>

					<li>
						<p> Since we have three terms, and the exponent on one term (<sq>
								<m>4</m>
							</sq> on <m>t^4</m>) is exactly
							twice the exponent on the other (<sq>
								<m>2</m>
							</sq> on <m>t^2</m>), we have a
							Quadratic in Disguise. We proceed accordingly.<me>\begin{array}{rclr}
							2t^4 &amp; = &amp; 9t^2 + 5 &amp; \\

								2t^4 - 9t^2 - 5 &amp; = &amp; 0 &amp; \text{Subtract $9t^2$ and $5$}
							\\
								(2t^2 + 1)(t^2 - 5) &amp; = &amp; 0 &amp; \text{Factor} \\
								2t^2 + 1 = 0 &amp; \text{or} &amp; t^2 = 5 &amp; \text{Zero Product
							Property} \\
								\end{array}</me> From <m>2t^2 + 1 = 0</m> we get <m>2t^2 = -1</m>,
							or <m>t^2 = -\frac{1}{2}</m>. We extract square roots as follows: <me>t
							= \pm \sqrt{-\dfrac{1}{2}} = \pm i \sqrt{\dfrac{1}{2}} = \pm i
							\dfrac{\sqrt{1}}{\sqrt{2}} = \pm i \dfrac{1}{\sqrt{2}} = \pm \dfrac{i
							\sqrt{2}}{2},</me> where we have rationalized the denominator per
							convention. From <m>t^2 = 5</m>, we get <m>t = \pm \sqrt{5}</m>. In
							total, we have four complex solutions - two real: <m>t = \pm \sqrt{5}</m>
							and two non-real: <m>t = \pm \frac{i \sqrt{2}}{2}</m>. </p>
					</li>

					<li>
						<p> To find the <em>real</em> solutions to <m>z^3 + 1 = 0</m>, we can
							subtract the <m>1</m> from both sides and extract cube roots: <m>z^3 =
							-1</m>, so <m>z = \sqrt[3]{-1} = -1</m>. It turns out there are two more
							non-real complex number solutions to this equation. To get at these, we
							factor:<me>\begin{array}{rclr}

								z ^ 3 + 1 &amp; = &amp; 0 &amp; \\
								(z + 1)(z^2 - z + 1) &amp; = &amp; 0 &amp; \text{Factor (Sum of Two
							Cubes)} \\
								z + 1 = 0 &amp; \text{or} &amp; z^2 - z + 1 = 0 &amp; \\
								\end{array}</me> From <m>z+1 = 0</m>, we get our real solution <m>z
							= -1</m>. From <m>z^2 -z + 1 = 0</m>, we apply the Quadratic Formula to
							get: <me>z = \dfrac{-(-1) \pm \sqrt{(-1)^2 - 4(1)(1)}}{2(1)} = \dfrac{1
							\pm \sqrt{-3}}{2} = \dfrac{1 \pm i\sqrt{3}}{2}</me> Thus we get <em>
							three</em> solutions to <m>z^3 + 1 = 0</m> - one real: <m>z = -1</m> and
							two non-real: <m>z = \frac{1 \pm i\sqrt{3}}{2}</m>. As always, the
							reader is encouraged to test their algebraic mettle and check these
							solutions. </p>
					</li>

				</ol>
			</p>
		</solution>
	</example>
	<p> It is no coincidence that the non-real solutions to the equations in Example <xref
			ref="complexsolnsreviewex" /> appear in complex conjugate pairs. Any time we use the
		Quadratic Formula to solve an equation with coefficients, the answers will form a complex
		conjugate pair owing to the <m>\pm</m> in the Quadratic Formula. </p>

	<!-- div attr= class="theorem1"-->
	<p> Discriminant Theorem Given a Quadratic Equation <m>ax^2 + bx + c = 0</m>, where <m>a</m>, <m>
		b</m> and <m>c</m> are real numbers, let <m>D = b^2 - 4ac</m> be the discriminant. </p>

	<p>
		<ul>
			<li>
				<p> If <m>D &gt; 0</m>, there are two distinct real number solutions to the
					equation. </p>
			</li>

			<li>
				<p> If <m>D = 0</m>, there is one (repeated) real number solution. </p>

				<p>
					<sq>Repeated</sq> here comes from the fact that <sq>both</sq> solutions <m>\frac{-b
					\pm 0}{2a}</m> reduce to <m>-\frac{b}{2a}</m>. </p>
			</li>

			<li>
				<p> If <m>D &lt; 0</m>, there are two non-real solutions which form a complex
					conjugate pair. </p>
			</li>

		</ul>
	</p><!--</div
	attr= class="theorem1">-->
</section>



