<?xml version="1.0" encoding="UTF-8" ?>
<!-- Generated by Pandoc using pretext.lua -->



	<section xml:id="intfactor-section">
		<title>Linear equations and the integrating factor</title>

		<p>
			One of the most important types of equations we will learn how to solve are the so-called <em>linear equations</em>. In fact, the majority of the course is about linear equations. In this section we focus on the <em></em>.
		</p>

<!-- div attr= class="definition"-->
		<p>
			A first order equation is <em>linear</em> if we can put it into the form: 
<men xml:id="lineq-eq1">
 y' + p(x) y = f(x) .
</men>
		</p><!--</div attr= class="definition">-->

		<p>
			The word means linear in <m>y</m> and <m>y'</m>; no higher powers nor functions of <m>y</m> or <m>y'</m> appear. The dependence on <m>x</m> can be more complicated.
		</p>

		<p>
			Solutions of linear equations have nice properties. For example, the solution exists wherever <m>p(x)</m> and <m>f(x)</m> are defined, and has the same regularity (read: it is just as nice). Weâ€™ll see this in detail in . But most importantly for us right now, there is a method for solving linear first order equations. In , we saw that we could easily solve equations of the form <me>\frac{dy}{dx} = f(x)</me> because we could directly integrate both sides of the equation, since the left hand side was the derivative of something (in this case, <m>y</m>) and the right side was only a function of <m>x</m>. We want to do the same here, but the something on the left will not be the derivative of just <m>y</m>.
		</p>

		<p>
			The trick is to rewrite the left-hand side of <xref ref="lineq-eq1" /> as a derivative of a product of <m>y</m> with another function. Let <m>r(x)</m> be this other function, and we can compute, by the product rule, that 
<me>
\frac{d}{dx}\Bigl[r(x)y\Bigr] = r(x)y' + r'(x) y.
</me>
 Now, if we multiply <xref ref="lineq-eq1" /> by the function <m>r(x)</m> on both sides, we get 
<me>
r(x)y' + p(x)r(x)y = f(x)r(x)
</me>
 and the first term on the left here matches the first term from our product rule derivative. To make the second terms match up as well, we need that 
<me>
r'(x) = p(x)r(x).
</me>
 This equation is separable! We can solve for the <m>r(x)</m> here by separating variables to get that 
<me>
\frac{dr}{r} = p(x)\, dx
</me>
 so that 
<me>
\ln{|r|} = \int p(x)\, dx
</me>
 or 
<me>
r(x) = e^{\int p(x) \,dx} .
</me>

		</p>

		<p>
			With this choice of <m>r(x)</m>, we get that 
<me>
r(x) y' + r(x) p(x) y = \frac{d}{dx}\Bigl[ r(x) y \Bigr], 
</me>
 so that if we multiply <xref ref="lineq-eq1" /> by <m>r(x)</m>, we obtain <m>r(x) y' + r(x) p(x) y</m> on the left-hand side, which we can simplify using our product rule derivative above to obtain 
<me>
 \frac{d}{dx}\Bigl[ r(x) y \Bigr] = r(x)f(x) .
</me>
 Now we integrate both sides. The right-hand side does not depend on <m>y</m> and the left-hand side is written as a derivative of a function. Afterwards, we solve for <m>y</m>. The function <m>r(x)</m> is called the <em></em> and the method is called the <em></em>.
		</p>

		<p>
			This method works for any first order linear equation, no matter what <m>p(x)</m> and <m>f(x)</m> are. In general, we can compute: <me>\begin{align*}
y' + p(x) y &amp;= f(x) , \\
e^{\int p(x) \,dx} y' + e^{\int p(x) \,dx} p(x) y &amp; = e^{\int p(x) \,dx} f(x) , \\
\frac{d}{dx}\left[ e^{\int p(x) \,dx} y \right] &amp; = e^{\int p(x) \,dx} f(x) , \\
e^{\int p(x) \,dx} y &amp; = \int e^{\int p(x) \,dx} f(x) \,dx + C , \\
y &amp; = e^{-\int p(x) \,dx} \left( \int e^{\int p(x) \,dx} f(x) \,dx + C \right) .
\end{align*}</me>
		</p>

		<p>
			Advice: Do not try to remember the formula itself, that is way too hard. It is easier to remember the process and repeat it.
		</p>

		<p>
			Of course, to get a closed form formula for <m>y</m>, we need to be able to find a closed form formula for the integrals appearing above.
		</p>


<example>
<title> </title>
<statement>		<p>
			Solve 
<me>
y' + 2xy = e^{x-x^2}, \qquad y(0) = -1 .
</me>

		</p>
</statement>

<solution>		<p>
			First note that <m>p(x) = 2x</m> and <m>f(x) = e^{x-x^2}</m>. The integrating factor is <m>r(x) = e^{\int p(x)\, dx} = e^{x^2}</m>. We multiply both sides of the equation by <m>r(x)</m> to get <me>\begin{align*}
e^{x^2} y' + 2xe^{x^2}y &amp; = e^{x-x^2} e^{x^2} , \\
\frac{d}{dx} \left[ e^{x^2} y \right] &amp;= e^x .
\end{align*}</me> We integrate <me>\begin{align*}
e^{x^2} y &amp;= e^x +C , \\
y &amp;= e^{x-x^2} + C e^{-x^2} .
\end{align*}</me> Next, we solve for the initial condition <m>-1 = y(0) = 1 + C</m>, so <m>C=-2</m>. The solution is 
<me>
y = e^{x-x^2} - 2 e^{-x^2} .
</me>

		</p>
</solution>
</example>
		<p>
			Note that we do not care which antiderivative we take when computing <m>e^{\int p(x) dx}</m>. You can always add a constant of integration, but those constants will not matter in the end.
		</p>

<exercise>
<statement>
		<p>
			Try it! Add a constant of integration to the integral in the integrating factor and show that the solution you get in the end is the same as what we got above.
		</p>
</statement>

<answer>		<p>
			Since we cannot always evaluate the integrals in closed form, it is useful to know how to write the solution in definite integral form. A definite integral is something that you can plug into a computer or a calculator. Suppose we are given 
<me>
y' + p(x) y = f(x) , \qquad y(x_0) = y_0 .
</me>
 Look at the solution and write the integrals as definite integrals. 
<men xml:id="lei-defsol">
 \mybxbg{
~~
y(x) = e^{-\int_{x_0}^x p(s)\, ds} \left( \int_{x_0}^x e^{\int_{x_0}^t p(s)\, ds}
f(t) \,dt + y_0 \right).
~~
}
</men>
You should be careful to properly use dummy variables here. If you now plug such a formula into a computer or a calculator, it will be happy to give you numerical answers.
		</p>
</answer>
</exercise>

<exercise>
<statement>
		<p>
			Check that <m>y(x_0) = y_0</m> in formula <xref ref="lei-defsol" />.
		</p>
</statement>

</exercise>

<example>
<title> </title>
<statement>		<p>
			Solve the initial value problem 
<me>
ty' + 4y = t^2 - 1 \qquad y(1) = 3.
</me>

		</p>
</statement>

<solution>		<p>
			In order to solve this equation, we want to put the equation in standard form, which is 
<me>
y' + \frac{4}{t}y = t - \frac{1}{t}.
</me>
 In this form, the coefficient <m>p(t)</m> of <m>y</m> is <m>p(t) = \frac{4}{t}</m>, so that the integrating factor is <me>r(t) = e^{\int p(t)\ dt} = e^{\int \frac{4}{t}\ dt} = e^{4\ln(t)}.</me> Since <m>4\ln(t) = \ln(t^4)</m>, we have that <m>r(t) = t^4</m>. Multiplying both sides of the equation by <m>t^4</m> gives 
<me>
t^4y' + 4t^3 y = t^5 - t^3
</me>
 where the left hand side is <m>\frac{d}{dt}(t^4y)</m>. Therefore, we can integrate both sides of the equation in <m>t</m> to give 
<me>
t^4 y = \frac{t^6}{6} - \frac{t^4}{4} + C
</me>
 and we can solve out for <m>y</m> as 
<me>
y(t) = \frac{t^2}{6} - \frac{1}{4} + \frac{C}{t^4}.
</me>
 To solve for <m>C</m> using the initial condition, we plug in <m>t=1</m> to get that we need 
<me>
3 = \frac{1}{6} - \frac{1}{4} + C \qquad C = \frac{37}{12}.
</me>
 Therefore, the solution to the initial value problem is 
<me>
y(t) = \frac{t^2}{6} - \frac{1}{4} + \frac{37/12}{t^4}.
</me>

		</p>
</solution>
</example>

<example>
<title> </title>
<statement>		<p>
			Solve the initial value problem 
<me>
y' + 2xy = 3 \qquad y(0) = 4.
</me>

		</p>
</statement>

<solution>		<p>
			This equation is already in standard form. Since the coefficient of <m>y</m> is <m>p(x) = 2x</m>, we know that the integrating factor is 
<me>
r(x) = e^{\int p(x)\ dx} = e^{x^2}.
</me>
 We can multiply both sides of the equation by this integrating factor to give 
<me>
y'e^{x^2} + 2xe^{x^2}y = 3e^{x^2}
</me>
 and then want to integrate both sides. The left-hand side of the equation is <m>\frac{d}{dx}[e^{x^2}y]</m>, so the antiderivative of that side is just <m>ye^{x^2}</m>. For the right-hand side, we would need to compute <me>\int 3e^{x^2}\ dx,</me> which does not have a closed-form expression. Therefore, we need to represent this as a definite integral. Since our initial condition gives the value of <m>y</m> at zero, we want to use zero as the bottom limit of the integral. Therefore, we can write the solution as <me>ye^{x^2} = \int_0^x 3e^{s^2}\ ds + C</me> and so can solve for <m>y</m> as 
<me>
y(x) = e^{-x^2} \int_0^x 3e^{s^2}\ ds + Ce^{-x^2}.
</me>
 Plugging in the initial condition gives that 
<me>
y(0) = 4 = e^{-0} \int_0^0 3e^{s^2}\ ds + Ce^{-0} = C.
</me>
 Therefore, the solution to the initial value problem is 
<me>
y(x) = e^{-x^2} \int_0^x 3e^{s^2}\ ds + 4e^{-x^2}.
</me>

		</p>
</solution>
</example>
<exercise>
<statement>
		<p>
			Write the solution of the following problem as a definite integral, but try to simplify as far as you can. You will not be able to find the solution in closed form. 
<me>
y' + y = e^{x^2-x}, \qquad y(0) = 10 .
</me>

		</p>
</statement>

<answer>		<p>
			 <m>y = e^{-x}\int_0^x e^{-s^2}\ ds + 10e^{-x}</m> 
		</p>
</answer>
</exercise>


<exercises>
			<title>Exercises</title>
<introduction>
			<p>
				In the exercises, feel free to leave answer as a definite integral if a closed form solution cannot be found. If you can find a closed form solution, you should give that.
			</p>
		</introduction>
<exercise>
<statement>
			<p>
				Solve <m>y' + xy = x</m>.
			</p>
</statement>

<answer>			<p>
				 <m>y = 1 + Ce^{-x^2}{2}</m> 
			</p>
</answer>
</exercise>

<exercise>
<statement>
			<p>
				Solve <m>y' + 6y = e^x</m>.
			</p>
</statement>

<answer>			<p>
				 <m>y = \frac{1}{7}e^x + Ce^{-6x}</m> 
			</p>
</answer>
</exercise>

<exercise>
<statement>
			<p>
				Solve <m>y' + 4y = x^2e^{-4x}</m>.
			</p>
</statement>

<answer>			<p>
				 <m>y = \frac{1}{3}x^3e^{-4x} + Ce^{-4x}</m> 
			</p>
</answer>
</exercise>

<exercise>
<statement>
			<p>
				Solve <m>y' - 3y = xe^x</m>.
			</p>
</statement>

<answer>			<p>
				 <m>y = -\frac{1}{2}xe^{x} - \frac{1}{4}e^x + Ce^{3x}</m> 
			</p>
</answer>
</exercise>

<exercise>
<statement>
			<p>
				Solve <m>y' + 3y = e^{4x} - e^{-2x}</m> with <m>y(0) = -3</m>.
			</p>
</statement>

<answer>			<p>
				 <m>y = \frac{1}{7}e^{4x} - e^{-2} + \frac{27}{7}e^{-3x}</m> 
			</p>
</answer>
</exercise>

<exercise>
<statement>
			<p>
				Solve <m>y' - 2y = x + 4</m>.
			</p>
</statement>

<answer>			<p>
				 <m>y = -\frac{x}{2} - \frac{9}{4} + Ce^{2x}</m> 
			</p>
</answer>
</exercise>

<exercise>
<statement>
			<p>
				Solve <m>xy' + 4y = x^2 - \frac{1}{x^2}</m>.
			</p>
</statement>

<answer>			<p>
				 <m>y = \frac{x^2}{6} - \frac{1}{2x^2} + Cx^{-4}</m> 
			</p>
</answer>
</exercise>

<exercise>
<statement>
			<p>
				Solve <m>xy' - 3y = x-2</m> with <m>y(1) = 3</m>.
			</p>
</statement>

<answer>			<p>
				 <m>y = -\frac{1}{2}x - \frac{2}{3} + \frac{25}{6}x^3</m> 
			</p>
</answer>
</exercise>

<exercise>
<statement>
			<p>
				Solve <m>y' - 4y = \cos{(3t)}</m>.
			</p>
</statement>

<answer>			<p>
				 <m>y = \frac{3}{25}\sin(3t) - \frac{4}{25}\cos(3t) + Ce^{4t}</m> 
			</p>
</answer>
</exercise>

<exercise>
<statement>
			<p>
				Solve <m>y'+3 x^2 y = x^2</m>.
			</p>
</statement>

</exercise>
<exercise>
<statement>
			<p>
				Solve <m>y' + 3x^2y = \sin(x) \, e^{-x^3}</m>, with <m>y(0) = 1</m>.
			</p>
</statement>

<answer>			<p>
				 <m>y = (2-\cos(x))e^{-x^3}</m> 
			</p>
</answer>
</exercise>

<exercise>
<statement>
			<p>
				Solve <m>y' + \cos (x) y = \cos(x)</m>.
			</p>
</statement>

<answer>			<p>
				 <m>y = 1 + Ce^{-\sin(x)}</m> 
			</p>
</answer>
</exercise>

<exercise>
<statement>
			<p>
				Solve the IVP <m>4ty'+y=24\sqrt{t};\ y(10000)=100.</m>
			</p>
</statement>

<answer>			<p>
				 <m>y = 8\sqrt{t} - 7000t^{-1/4}</m> 
			</p>
</answer>
</exercise>

<exercise>
<statement>
			<p>
				Solve the IVP <m>(t^2+1)y' - 2ty = t^2+1; \ y(1)=0</m>.
			</p>
</statement>

<answer>			<p>
				 <m>y = (t^2 + 1)\left(\tan^{-1}(t) - \frac{\pi}{4}\right)</m> 
			</p>
</answer>
</exercise>

<exercise>
<statement>
			<p>
				Solve <m>\frac{1}{x^2+1} \, y' + x y = 3</m>, with <m>y(0) = 0</m>.
			</p>
</statement>

<answer>			<p>
				 <m>y = e^{-\left(\frac{x^4}{4} + \frac{x^2}{2}\right)}\int_0^x 3e^{\frac{s^4}{4} + \frac{s^2}{2}}(s^2 + 1)\ ds</m> 
			</p>
</answer>
</exercise>

<exercise>
<statement>
			<p>
				Solve <m>y'+ 2\sin(2x) y = 2\sin(2x)</m>, <m>y(\nicefrac{\pi}{2}) = 3</m>.
			</p>
</statement>

</exercise>
<exercise>
<statement>
			<p>
				Consider the initial value problem <me>5y' - 3y = e^{-2t} \qquad y(0) = a</me> for an undetermined value <m>a</m>. Solve the problem and determine the dependence on the value of <m>a</m>. How does the value of the solution as <m>t \rightarrow \infty</m> depend on the value of <m>a</m>?
			</p>
</statement>

<answer>			<p>
				 <m>y = -\frac{1}{13}e^{-2t} + \left(a + \frac{1}{13}\right)e^{3/5}t</m>. If <m>a &gt; -\frac{1}{13}</m>, the solution goes to <m>\infty</m>, if <m>a = -\frac{1}{13}</m>, the solution goes to 0, if <m>a &lt; -\frac{1}{13}</m>, the solution goes to <m>-\infty</m>. 
			</p>
</answer>
</exercise>

<exercise>
<statement>
			<p>
				Find an expression for the general solution to <m>y' + 3y = \sin(t^2)</m> with <m>y(0) = 2</m>. Simplfy your answer as much as possible.
			</p>
</statement>

<answer>			<p>
				 <m>y = 2e^{-3t} + e^{-3t}\int_0^t e^{3s}\sin(s^2)\ ds</m> 
			</p>
</answer>
</exercise>
</exercises>

	</section>



